Clean.lean
@@ -2,6 +2,7 @@ import Clean.Caliper.MultiLimbCompile
 import Clean.Caliper.MultiLimbOps
 import Clean.Caliper.RegOnly
 import Clean.Caliper.MultiLimbInv
+import Clean.Caliper.MultiLimbIR
 import Clean.Caliper.MultiLimb
 import Clean.Caliper.WitgenCompile
 import Clean.Caliper.WitgenComputable
